Update with rough sketch of DTM instance and repr theorem

Tealeaves/Adapters/Isomorphisms/BatchtoKStore.v
@@ -2,11 +2,18 @@ From Tealeaves Require Export
   Functors.Batch
   Functors.KStore.
 
+Import Batch.Notations.
+Import Applicative.Notations.
+
+About length_Batch.
+#[local] Arguments length_Batch {A B C}%type_scope b.
+
 (** * Batch to KStore *)
 (******************************************************************************)
 Section batch_to.
 
-  Context (A B C : Type).
+
+  Context {A B C : Type}.
 
   Definition Batch_to_Vector:
     Batch A B C -> @sigT nat (Vector.t A).
@@ -33,7 +40,7 @@ Section batch_to.
         apply mk.
         assumption.
         assumption.
-  Qed.
+  Defined.
 
   Definition deconstruct_Batch:
     Batch A B C -> @sigT nat (fun n => VEC n A * (VEC n B -> C)).
@@ -60,7 +67,156 @@ Section batch_to.
     eapply (runBatch (KStore A B) kstore).
   Defined.
 
+  Definition Batch_to_Vector'
+    (b: Batch A B C): Vector.t A (length_Batch b).
+  Proof.
+    induction b.
+    - apply Vector.nil.
+    - cbn.
+      apply Vector.cons;
+      assumption.
+  Defined.
+
+  Definition Batch_to_makeFn'
+    (b: Batch A B C): Vector.t B (length_Batch b) -> C.
+  Proof.
+    induction b.
+    - intros ?; assumption.
+    - cbn.
+      intro X.
+      apply VectorDef.uncons in X.
+      destruct X.
+      apply IHb; auto.
+  Defined.
+
+  Definition Batch_to_Vector''
+    (b: Batch A B C): Vector.t A (length_Batch b).
+  Proof.
+    induction b.
+    - apply Vector.nil.
+    - cbn.
+      apply Vector.cons;
+      assumption.
+  Defined.
+
+  Definition Batch_to_makeFn''
+    (b: Batch A B C): Vector.t B (length_Batch b) -> C.
+  Proof.
+    induction b.
+    - intros ?; assumption.
+    - cbn.
+      intro X.
+      apply VectorDef.uncons in X.
+      destruct X.
+      apply IHb; auto.
+  Defined.
+
 End batch_to.
+
+Lemma Batch_to_Vector_step {A B C}: forall (a: A) (b: Batch A B (B -> C)),
+    Batch_to_Vector' (b ⧆ a) =
+      Vector.cons A a (length_Batch b) (Batch_to_Vector' b).
+Proof.
+  reflexivity.
+Qed.
+
+Lemma Batch_to_makeFn_step {A B C}: forall (a: A) (b: Batch A B (B -> C)),
+    Batch_to_makeFn' (b ⧆ a) =
+      fun (v:Vector.t B (S (length_Batch b))) =>
+          match (Vector.uncons v) with
+          | (b', v') => Batch_to_makeFn' b v' b'
+          end.
+Proof.
+  reflexivity.
+Qed.
+
+From Tealeaves Require Import
+               Classes.Coalgebraic.TraversableFunctor
+               Adapters.KleisliToCoalgebraic.TraversableFunctor.
+
+Section aksdjflasdf.
+
+  Context
+   T (A:Type) G `{Applicative G}
+     `{Kleisli.TraversableFunctor.TraversableFunctor T}.
+
+  Definition toLen: forall (t : T A), nat.
+    intro t.
+    exact (length_Batch (B := A) (toBatch t)).
+  Defined.
+
+  Definition toMake: forall (t : T A),
+      Vector.t A (toLen t) -> (T A).
+  Proof.
+    intros t B.
+    unfold toLen.
+    apply (Batch_to_makeFn' (toBatch t)).
+    assumption.
+  Defined.
+
+  Definition toContents: forall (t : T A),
+      Vector.t A (toLen t).
+  Proof.
+    intro t.
+    unfold toLen.
+    apply (Batch_to_Vector' (toBatch t)).
+  Defined.
+
+  Definition toLen' (B:Type): forall (t : T A), nat.
+    intro t.
+    exact (length_Batch (B := B) (toBatch t)).
+  Defined.
+
+  Definition toMake' B: forall (t : T A),
+      Vector.t B (toLen' B t) -> (T B).
+  Proof.
+    intros t.
+    unfold toLen.
+    apply (Batch_to_makeFn' (toBatch t)).
+  Defined.
+
+  Definition toContents' B: forall (t : T A),
+      Vector.t A (toLen' B t).
+  Proof.
+    intro t.
+    apply (Batch_to_Vector' (toBatch t)).
+  Defined.
+
+
+  Lemma repr: forall `(t : T A),
+      t = toMake t (toContents t).
+  Proof.
+    intros.
+    unfold toMake, toContents.
+    change t with (id t) at 1.
+    rewrite <- trf_extract.
+    unfold compose at 1.
+    eapply (
+        Batch_ind A A
+                  (fun (T1 : Type) (b0 : Batch A A T1) =>
+                     extract_Batch b0 =
+                       Batch_to_makeFn' b0 (Batch_to_Vector' b0))).
+    - reflexivity.
+    - intros.
+      rewrite Batch_to_makeFn_step.
+      rewrite Batch_to_Vector_step.
+      cbn.
+      rewrite H5.
+      reflexivity.
+  Qed.
+
+  Lemma repr': forall `(t : T A) B (f : A -> G B),
+      traverse f t = pure (toMake' B t) <⋆>
+                       (traverse (T := VEC (toLen' B t)) f (toContents' B t)).
+  Proof.
+    intros.
+    unfold toMake', toContents'.
+    Search traverse toBatch.
+    rewrite traverse_through_runBatch.
+    unfold compose at 1.
+  Admitted.
+
+End aksdjflasdf.
 
 (** ** <<KStore>> to <<Batch>> *)
 (******************************************************************************)
@@ -110,6 +266,7 @@ Section toBatch.
 
 End toBatch.
 
+(*
 (* ISOS *)
 Section isos.
 
@@ -159,3 +316,8 @@ Section isos.
   cbv.
 
 End isos.
+<<<<<<< ours
+<<<<<<< Updated upstream
+=======
+*)
+
