Tealeaves/Examples/Lambda+VariadicLet/Syntax.v
@@ -12,7 +12,7 @@ Export Product.Notations. (* × *)
 Export ContainerFunctor.Notations. (* ∈ *)
 Export DecoratedContainerFunctor.Notations. (* ∈d *)
 
-#[local] Generalizable Variables G.
+#[local] Generalizable Variables G A B C.
 
 #[local] Set Implicit Arguments.
 
@@ -25,6 +25,83 @@ Inductive term (v : Type) :=
 
 #[export] Instance Return_Lam: Return term := tvar.
 
+Print term_rect.
+
+Section term_induction.
+
+  Variables
+    (v : Type)
+    (P : term v -> Prop).
+
+  Hypotheses
+    (tvar_case : forall v, P (tvar v))
+    (letin_nil_case :  forall t, P t -> P (letin nil t))
+    (letin_cons_case : forall (u: term v) (l : list (term v)) (t: term v)
+                         (IHu: P u) (IHl: List.Forall P l)
+                         (IHt: P t), P (letin (u :: l) t))
+    (app_case : forall t: term v, P t -> forall u: term v, P u -> P (app t u)).
+
+
+  Print term_rect.
+  #[program] Definition term_mut_ind: forall t, P t.
+  refine (fix F t := match t with
+          | tvar v => tvar_case v
+          | letin defs body =>
+              match defs with
+              | nil => @letin_nil_case body (F body)
+              | cons u rest =>
+                  @letin_cons_case u rest body
+                                   (F u) _ (F body)
+              end
+          | app t1 t2 =>
+              @app_case t1 (F t1) t2 (F t2)
+                     end).
+  admit.
+  Admitted.
+
+End term_induction.
+
+(*
+Section term_induction.
+
+  Variables
+    (v : Type)
+    (P : term v -> Type).
+
+  Hypotheses
+    (tvar_case : forall v, P (tvar v))
+    (letin_case : forall (l : list (term v)) (t : term v)
+                      (rec: forall t, t ∈ l -> P t),
+          P t -> P (letin l t))
+    (app_case : forall t: term v, P t -> forall u: term v, P u -> P (app t u)).
+
+
+  #[program] Definition term_mut_rect: forall t, P t.
+  refine (fix F t :=
+      match t with
+      | tvar v =>
+          tvar_case v
+      | letin defs body =>
+          @letin_case defs body
+                      ((fix G (ls : list (term v)): forall t, t ∈ ls -> P t :=
+                          match ls with
+                          | nil => _
+                          | cons x rest => _
+                          end
+                       ) defs)
+                      (F body)
+      | app t u =>
+          @app_case t (F t) u (F u)
+      end).
+  - inversion 1.
+  - intros t' t_in.
+    cbn in t_in.
+    admit.
+  Admitted.
+
+End term_induction.
+*)
+
 Fixpoint binddt_term
            (G : Type -> Type) `{Map G} `{Pure G} `{Mult G}
            {v1 v2 : Type}
@@ -32,763 +109,125 @@ Fixpoint binddt_term
            (t : term v1) : G (term v2) :=
   match t with
   | tvar v => f (0, v)
-  | letin body => pure (lam τ) <⋆> binddt_term (preincr f 1) body
-  | app t1 t2 => pure (@app v2) <⋆> binddt_term f t1 <⋆> binddt_term f t2
+  | letin defs body =>
+      pure (@letin v2) <⋆>
+      ((fix F ls :=
+      match ls with
+      | nil => pure nil
+      | cons d0 drest =>
+          pure cons <⋆> binddt_term f d0 <⋆> F drest
+      end) defs) <⋆> binddt_term (f ⦿ length defs) body
+  | app t1 t2 =>
+      pure (@app v2) <⋆> binddt_term f t1 <⋆> binddt_term f t2
   end.
 
 #[export] Instance Binddt_Lam: Binddt nat term term := @binddt_term.
 
-(*|
-========================================
-Some rewriting principles for binddt
-========================================
-
-These definitional equalities help prove the composition law later.
-
-|*)
-
-Section binddt_helpers.
-
-  Generalizable Variable F.
-  Context
-    `{Applicative F}
-      {v1 v2 v3 : Type}
-      (f : nat * v1 -> F (term v2)).
-
-  Notation "'P'" := pure.
-  Notation "'BD'" := binddt.
-
-  Lemma binddt_lam :
-    forall (τ : typ), BD f ∘ (@lam v1 τ) = (precompose (BD (preincr f 1)) ∘ ap F ∘ P) (@lam v2 τ).
-  Proof.
+Lemma binddt_rw_letin: forall `{Applicative G} (v1 v2 : Type)
+                         (l : list (term v1)) (body: term v1),
+  forall f : nat * v1 -> G (term v2),
+    binddt_term f (letin l body) =
+      pure (@letin v2) <⋆> traverse (binddt_term f) l <⋆>
+        binddt_term (f ⦿ length l) body.
+Proof.
+  intros.
+  destruct l.
+  - cbn.
+    change 0 with (Ƶ:nat).
+    rewrite preincr_zero.
     reflexivity.
-  Qed.
+  - cbn.
+    repeat fequal.
+    induction l.
+    + reflexivity.
+    + cbn. rewrite IHl.
+      reflexivity.
+Qed.
 
-  Lemma binddt_app :
-      compose (BD f) ∘ @app v1 = (compose (precompose (BD f) ∘ ap F) ∘ precompose (BD f) ∘ ap F ∘ P) (@app v2).
-  Proof.
+Lemma binddt_helper_letin
+        `{Applicative G1}
+        `{Applicative G2}
+        A B C
+    (f : nat * A -> G1 (term B))
+    (g : nat * B -> G2 (term C)):
+    pure (compose (binddt_term g) ∘ letin (v:=B)) =
+      pure (compose (binddt_term g) ∘ letin (v:=B)).
+Proof.
+  unfold compose.
+Abort.
+
+Theorem dtm1_lam:
+  forall `{Applicative G} (A B : Type),
+  forall f : nat * A -> G (term B),
+    binddt f ∘ ret  = f ∘ ret (T := (nat ×)).
+Proof.
+  reflexivity.
+Qed.
+
+Theorem dtm2_term : forall A : Type,
+    binddt (T := term) (U := term)
+           (G := fun A => A) (ret (T := term) ∘ extract (W := (nat ×))) = @id (term A).
+Proof.
+  intros. ext t. unfold id.
+  induction t using term_mut_ind.
+  - cbn. reflexivity.
+  - cbn.
+    change 0 with (Ƶ:nat).
+    rewrite preincr_zero.
+    rewrite IHt.
     reflexivity.
-  Qed.
+  - cbn.
+    rewrite extract_preincr2.
+Admitted.
 
-End binddt_helpers.
+Theorem dtm3_term:
+  forall `{Applicative G1} `{Applicative G2},
+  forall `(g : nat * B -> G2 (term C)) `(f : nat * A -> G1 (term B)),
+    map (binddt_term g) ∘ binddt_term f = binddt_term (G := G1 ∘ G2) (g ⋆7 f).
+Proof.
+  intros. ext t.
+  generalize dependent g.
+  generalize dependent f.
+  unfold compose at 1.
+  induction t; intros f g.
+  - cbn. change (preincr g 0) with (preincr g Ƶ).
+    now rewrite preincr_zero.
+  - specialize (IHt (f ⦿ length l) (g ⦿ length l)).
+    rewrite kc7_preincr in IHt.
+    (* left *)
+    rewrite binddt_rw_letin.
+    rewrite map_ap.
+    rewrite map_ap.
+    rewrite app_pure_natural.
+    (* right *)
+    rewrite binddt_rw_letin.
 
-(*|
-========================================
-An overview of the DTM axioms
-========================================
-|*)
-
-Section laws.
-
-  (* Generalize over (Coq) variables used for object-level variables
-   and symbols for applicative homomorphisms. *)
-  Generalizable Variables v ϕ.
-
-  Ltac rewrite_with_bind_hyp :=
-    match goal with
-    | H : context[binddt] |- _ => rewrite H
-    end.
-
-  Ltac induction_on_term :=
-    match goal with
-    | t : term ?v |- _ => induction t
-    end.
-
-  Ltac dtm_setup :=
-    intros; ext t; unfold id; induction_on_term; cbn.
-
-(*|
-~~~~~~~~~~~~~~~~~~~~~~~~~~~~~~~~~~~~~~~~~~
-Composition with unit (left unit law)
-~~~~~~~~~~~~~~~~~~~~~~~~~~~~~~~~~~~~~~~~~~
-
-The "composition with unit" law (or left unit law) establishes that
-the atomic expression `ret term v`
-
-1. consists just of variable `v`
-2. inside an empty binding context
-
-In this law, `ret (list β ×)` is the operation which lifts any `v`
-into an empty binding context to get `([], v)`. A simpler way of
-writing the left unit law is then
-
-`binddt f (ret term v) = f ([], v)`
-
-The proof of this rule ought to follow merely from the definitions of
-`binddt` and `ret`.  In the course of proofs about `binddt f t` by
-induction of the syntax of expression `t`, the left unit law acts as
-a base case.
-
-.. coq::
-   :name: dtm1
-|*)
-  Ltac solve_dtm1 :=
-    intros; now try ext var.
-
-  Theorem dtm1_stlc:
-    forall `{Applicative G} (A B : Type),
-       forall f : nat * A -> G (term B),
-         binddt f ∘ ret  = f ∘ ret (T := (nat ×)).
-  Proof.
-    reflexivity.
-  Qed.
-
-(*|
-~~~~~~~~~~~~~~~~~~~~~~~~~~~~~
-Identity law (right unit law)
-~~~~~~~~~~~~~~~~~~~~~~~~~~~~~
-
-The identity law (or right unit law) establishes that applying the
-substitution rule
-
-`pure F ∘ ret term ∘ extract ((list β) ×)`
-
-to each of the variables in expression `t` acts as the pure effect on
-`t`. The substitution rule is the one which at each variable
-
-1. throws away the binding context: `list β * v -> v`
-2. coerces the variable into an atomic expression: `v -> term v`
-3. and lifts the result into `F` with the `pure` effect: `term v -> F (term v)`
-
-.. coq::
-   :name: dtm2
-|*)
-
-  Generalizable All Variables.
-
-  Lemma dtm2_helper : forall `{Monoid M} (m : M) `(f : A -> B),
-      preincr (f ∘ extract) m = f ∘ extract.
-  Proof.
-    intros. unfold preincr. reassociate ->. now rewrite (extract_incr).
-  Qed.
-
-  Theorem dtm2_stlc : forall A : Type, binddt (T := term) (U := term)
-                                    (G := fun A => A) (ret (T := term) ∘ extract (W := (nat ×))) = @id (term A).
-  Proof.
-    intros. ext t. unfold id.
-    induction t.
-    - cbn. fequal.
-    - cbn. fequal; (rewrite dtm2_helper; auto).
-    - cbn. fequal; auto.
-  Qed.
-
-  Ltac solve_dtm2_case :=
-    fequal; repeat rewrite dtm2_helper; auto.
-
-  Theorem dtm2_stlc_automated : forall A : Type, binddt (G := fun A => A) (T := term) (ret (T := term) ∘ extract (W := (nat ×))) = @id (term A).
-    dtm_setup; solve_dtm2_case.
-  Qed.
-
-(*|
-~~~~~~~~~~~~~~~~~~~~~~~~
-Composition law
-~~~~~~~~~~~~~~~~~~~~~~~~
-
-The composition law states the following:
-
-`map F (binddt g) ∘ binddt f = binddt (g ⋆ f)`
-
-The right-hand side may be written more explicitly as
-
-`binddt (fun '(w, x) => map F (binddt (F := G) (g ∘ incr w)) (f (w, x))))`
-
-This law is an analogue of the ordinary monad composition law
-
-`bind g ∘ bind f = bind (bind g ∘ f)`.
-
-Both are loosely of the form
-
-`bind g ∘ bind f = bind (g ∗ f)`
-
-A close comparison shows the rules differ in two respects:
-
-1. The call to `g` in `bind g` is replaced with a call to `(g ∘ incr
-   w)` where `w` is the context seen by the function `f`.
-2. The call to `binddt (g ∘ incr w)` is wrapped in `map F`. This is
-   required to map over the applicative effect of type `F` generated
-   by the application of `f`.
-
-.. coq::
-   :name: dtm3
-|*)
-
-  Notation "'P'" := pure.
-  Notation "'F'" := map.
-  Notation "'BD'" := (binddt term).
-
-  Ltac dtm3_lhs_step G1 :=
-    repeat rewrite map_ap; (* Bring LHS <<map>> up to the constructor *)
-    rewrite (app_pure_natural (G := G1)). (* Fuse <<map>> and the <<pure (constructor)>> *)
-
-  Ltac dtm3_rhs_step G2 G1 :=
-    (rewrite_strat innermost (terms (ap_compose2 G2 G1)));
-    repeat rewrite map_ap;
-    rewrite (app_pure_natural (G := G1));
-    rewrite <- ap_map;
-    repeat rewrite map_ap;
-    rewrite (app_pure_natural (G := G1)).
-
-  Set Keyed Unification.
-
-  Theorem dtm3_stlc :
-    forall `{Applicative G1} `{Applicative G2},
-        forall `(g : nat * B -> G2 (term C)) `(f : nat * A -> G1 (term B)),
-          map (binddt g) ∘ binddt f = binddt (G := G1 ∘ G2) (g ⋆7 f).
-  Proof.
-    intros. ext t.
-    generalize dependent g.
-    generalize dependent f.
+    Set Keyed Unification.
+    rewrite <- IHt.
     unfold compose at 1.
-    induction t; intros f g.
-    - cbn. change (preincr g 0) with (preincr g Ƶ).
-      now rewrite preincr_zero.
-    - cbn.
-      rewrite <- (kc7_preincr).
-      rewrite <- IHt.
-      (* left side *)
-      repeat rewrite map_ap. (* Bring LHS <<map>> up to the constructor *)
-      rewrite (app_pure_natural). (* Fuse <<map>> and the <<pure (constructor)>> *)
-      (* right side, constructor *)
-      unfold_ops @Pure_compose.
-      (* right side, first argument *)
-      rewrite_strat innermost (terms (ap_compose2 G2 G1)).
-      rewrite (app_pure_natural).
-      rewrite <- ap_map.
-      rewrite (app_pure_natural).
-      reflexivity.
-    - cbn.
-      rewrite <- IHt1.
-      rewrite <- IHt2.
-      (* left side *)
-      do 2 rewrite map_ap.
-      rewrite (app_pure_natural).
-      (* right side *)
-      (* right side, constructor *)
-      unfold_ops @Pure_compose.
-      (* right side, first argument *)
-      rewrite_strat innermost (terms (ap_compose2 G2 G1)).
-      repeat rewrite map_ap.
-      rewrite (app_pure_natural).
-      rewrite <- ap_map.
-      repeat rewrite map_ap.
-      rewrite (app_pure_natural).
-      (* right side, second argument *)
-      rewrite_strat innermost (terms (ap_compose2 G2 G1)).
-      repeat rewrite map_ap.
-      rewrite (app_pure_natural).
-      rewrite <- ap_map.
-      repeat rewrite map_ap.
-      rewrite (app_pure_natural).
-      reflexivity.
-  Qed.
+Abort.
 
-  Theorem dtm3_stlc_automated :
-    forall (A B C : Type) (G1 : Type -> Type) (H1 : Map G1) (H2 : Pure G1) (H3 : Mult G1),
-      Applicative G1 ->
-      forall (G2 : Type -> Type) (H5 : Map G2) (H6 : Pure G2) (H7 : Mult G2),
-        Applicative G2 ->
-        forall (g : nat * B -> G2 (term C)) (f : nat * A -> G1 (term B)),
-          map (binddt g) ∘ binddt f = binddt (G := G1 ∘ G2) (g ⋆7 f).
-  Proof.
-    intros. ext t.
-    unfold compose at 1.
-    generalize dependent g.
-    generalize dependent f.
-    induction_on_term; intros f g.
-    - cbn. change (preincr g 0) with (preincr g Ƶ).
-      now rewrite preincr_zero.
-    - cbn.
-      rewrite <- (kc7_preincr g f).
-      rewrite <- IHt.
-      dtm3_lhs_step G1.
-      dtm3_rhs_step G2 G1.
-      reflexivity.
-    - cbn.
-      dtm3_lhs_step G1.
-      rewrite <- IHt1.
-      rewrite <- IHt2.
-      dtm3_rhs_step G2 G1.
-      dtm3_rhs_step G2 G1.
-      reflexivity.
-  Qed.
-
-(*|
-~~~~~~~~~~~~~~~~~~~~~~~~~~~~~~~~~~~~~~~~~~
-Applicative homomorphism law
-~~~~~~~~~~~~~~~~~~~~~~~~~~~~~~~~~~~~~~~~~~
-
-This law states that `binddt` is parametric with respect to
-applicative functors in the sense that it commutes with their
-homomorphisms. It is (probably?) a free theorem, so it is not actually
-a restriction on implementations of `binddt` (cite Gibbons).
-
-
-.. coq::
-   :name: dtm4
-|*)
-
-  Theorem dtm4_stlc :
-    forall (G1 G2 : Type -> Type) (H1 : Map G1) (H2 : Mult G1) (H3 : Pure G1) (H4 : Map G2) (H5 : Mult G2) (H6 : Pure G2)
-      (ϕ : forall A : Type, G1 A -> G2 A), ApplicativeMorphism G1 G2 ϕ ->
-      forall (A B : Type) (f : nat * A -> G1 (term B)),
-        ϕ (term B) ∘ binddt f = binddt (ϕ (term B) ∘ f).
-  Proof.
-    intros. ext t.
-    inversion H.
-    generalize dependent f.
-    unfold compose at 1.
-    induction t; intro f. (* .unfold *)
-    - reflexivity.
-    - cbn.
-      repeat rewrite ap_morphism_1.
-      rewrite appmor_pure.
-      rewrite IHt.
-      reflexivity.
-    - cbn.
-      repeat rewrite ap_morphism_1.
-      rewrite appmor_pure.
-      rewrite IHt1.
-      rewrite IHt2.
-      reflexivity.
-  Qed.
-
-  Theorem dtm4_automated :
-    forall (G1 G2 : Type -> Type) (H1 : Map G1) (H2 : Pure G1) (H3 : Mult G1) (H4 : Map G2) (H5 : Pure G2) (H6 : Mult G2)
-      (ϕ : forall A : Type, G1 A -> G2 A),
-      ApplicativeMorphism G1 G2 ϕ ->
-      forall (A B : Type) (f : nat * A -> G1 (term B)),
-        ϕ (term B) ∘ binddt f = binddt (ϕ (term B) ∘ f).
-  Proof.
-    intros. ext t.
-    inversion H.
-    unfold compose at 1.
-    generalize dependent f.
-    induction t; intro f; cbn.
-    - reflexivity.
-    - repeat rewrite ap_morphism_1.
-      rewrite appmor_pure.
-      rewrite IHt.
-      reflexivity.
-    - repeat rewrite ap_morphism_1.
-      rewrite appmor_pure.
-      rewrite IHt1.
-      rewrite IHt2.
-      reflexivity.
-  Qed.
-
-  #[export] Instance DTMPre_Lam:
-    DecoratedTraversableRightPreModule nat term term :=
-    {| kdtm_binddt1 := dtm2_stlc;
-       kdtm_binddt2 := @dtm3_stlc;
-       kdtm_morph := @dtm4_stlc;
-    |}.
-
-  #[export] Instance DTM_Lam:
-    DecoratedTraversableMonad nat term :=
-    {| kdtm_binddt0 := @dtm1_stlc;
-    |}.
-
-  #[export] Instance Map_Lam: Map term
-    := Map_Binddt nat term term.
-  #[export] Instance Mapd_Lam: Mapd nat term
-    := Mapd_Binddt nat term term.
-  #[export] Instance Traverse_Lam: Traverse term
-    := Traverse_Binddt nat term term.
-  #[export] Instance Mapdt_Lam: Mapdt nat term
-    := Mapdt_Binddt nat term term.
-  #[export] Instance Bind_Lam: Bind term term
-    := Bind_Binddt nat term term.
-  #[export] Instance Bindd_Lam: Bindd nat term term
-    := Bindd_Binddt nat term term.
-  #[export] Instance Bindt_Lam: Bindt term term
-    := Bindt_Binddt nat term term.
-  #[export] Instance Elements_Lam: Elements term
-    := Elements_Traverse.
-
-  #[export] Instance DTMFull_Lam:
-    DecoratedTraversableMonadFull nat term
-    := DecoratedTraversableMonadFull_DecoratedTraversableMonad nat term.
-
-End laws.
-
-Section test_notations.
-
-  Context
-    (β : Type)
-    (x y z : atom)
-    (b : β) (τ : typ).
-
-  Check 1.
-  Check (λ τ (tvar (Bd 1))).
-  Check (λ τ (tvar (Fr x))).
-  Check [λ τ (tvar (Bd 1))]@[tvar (Fr x)].
-  Check [λ τ (tvar (Fr x))]@[tvar (Bd 0)].
-  Check λ τ ([(tvar (Bd 1))]@[tvar (Fr x)]).
-  Check λ τ ([(tvar (Fr x))]@[tvar (Bd 0)]).
-
-End test_notations.
-
-Definition ctx := list (atom * typ).
-
-Reserved Notation "Γ ⊢ t : S" (at level 90, t at level 99).
-
-Inductive Judgment : ctx -> term LN -> typ -> Prop :=
-| j_var :
-    forall (Γ : ctx) (x : atom) (A : typ),
-      uniq Γ ->
-      (x, A) ∈ Γ ->
-      Γ ⊢ tvar (Fr x) : A
-| j_abs :
-    forall (L : AtomSet.t) Γ (τ1 τ2 : typ) (t : term LN),
-      (forall x : atom, ~ AtomSet.In x L -> Γ ++ x ~ τ1 ⊢ t '(tvar (Fr x)) : τ2) ->
-      Γ ⊢ λ τ1 t : τ1 ⟹ τ2
-| j_app :
-    forall Γ (t1 t2 : term LN) (A B : typ),
-      Γ ⊢ t1 : A ⟹ B ->
-      Γ ⊢ t2 : A ->
-      Γ ⊢ [t1]@[t2] : B
-where "Γ ⊢ t : A" := (Judgment Γ t A).
-
-(** * Rewriting lemmas for high-level operations *)
-(******************************************************************************)
-
-Ltac simplify_to_monoid :=
-  unfold_ops @Pure_const @Mult_const; simpl_monoid.
-
-Ltac extract_preincr :=
-    match goal with
-      |- context[((?f ∘ extract) ⦿ ?w)] =>
-        rewrite extract_preincr2
-    end.
-
-(** ** Rewriting lemmas for <<tolist>>, <<toset>> *)
-(******************************************************************************)
-Section term_list_rewrite.
-
-  Variable
-    (A : Type).
-
-  Ltac solve_in_term :=
-    unfold_ops @Pure_const;
-    repeat rewrite (@map_const_spec (A -> Prop) _ _ (ret term));
-    simpl_monoid;
-    repeat rewrite (dtm2_helper);
-    try reflexivity.
-
-  Lemma tolist_term_1 : forall (x : A),
-    tolist (tvar x) = [x].
-  Proof.
-    reflexivity.
-  Qed.
-
-  Lemma map_const_rw: forall A B (f: A -> B) X,
-      map (F := const X) f = @id X.
-  Proof.
-    reflexivity.
-  Qed.
-
-  Lemma tolist_term_2 : forall (X : typ) (t : term A),
-    tolist (lam X t) = tolist t.
-  Proof.
-    intros.
-    cbn.
-    extract_preincr.
-    reflexivity.
-  Qed.
-
-  Lemma tolist_term_3 : forall (t1 t2 : term A),
-      tolist (app t1 t2) = tolist t1 ++ tolist t2.
-  Proof.
-    reflexivity.
-  Qed.
-
-  Lemma in_term_1 : forall (x y : A),
-      x ∈ tvar y <-> x = y.
-  Proof.
-    intros.
-    cbn.
-    cbv. intuition.
-  Qed.
-
-  Lemma in_term_2 : forall (y : A) (X : typ) (t : term A),
-    y ∈ (lam X t) <-> y ∈ t.
-  Proof.
-    intros. cbn. rewrite dtm2_helper.
-    unfold_ops @Pure_const; simpl_monoid.
-    reflexivity.
-  Qed.
-
-  Lemma in_term_3 : forall (t1 t2 : term A) (y : A),
-      y ∈ (app t1 t2) <-> y ∈ t1 \/ y ∈ t2.
-  Proof.
-    intros. cbn.
-    unfold_ops @Pure_const @Mult_const.
-    simpl_monoid.
-    reflexivity.
-  Qed.
-
-End term_list_rewrite.
-
-(** ** Rewriting lemmas for <<free>>, <<freeset>> *)
-(******************************************************************************)
-Section term_free_rewrite.
-
-  Variable (A : Type).
-
-  Lemma term_free11 : forall (b : nat) (x : atom),
-      x ∈ free (tvar (Bd b)) <-> False.
-  Proof.
-    intros. reflexivity.
-  Qed.
-
-  Lemma term_free12 : forall (y : atom) (x : atom),
-      x ∈ free (tvar (Fr y)) <-> x = y.
-  Proof.
-    intros. cbn.
-    intuition.
-  Qed.
-
-  Lemma term_free2 : forall (x : atom) (t : term LN) (X : typ),
-      x ∈ free (lam X t) <-> x ∈ free t.
-  Proof.
-    intros.
-    rewrite in_free_iff.
-    rewrite in_term_2.
-    now rewrite <- in_free_iff.
-  Qed.
-
-  Lemma term_free3 : forall (x : atom) (t1 t2 : term LN),
-      x ∈ free (app t1 t2) <-> x ∈ free t1 \/ x ∈ free t2.
-  Proof.
-    intros. rewrite in_free_iff. rewrite in_term_3.
-    now rewrite <- 2(in_free_iff).
-  Qed.
-
-  Lemma term_in_freeset11 : forall (b : nat) (x : atom),
-      AtomSet.In x (freeset (tvar (Bd b))) <-> False.
-  Proof.
-    intros. rewrite <- free_iff_freeset.
-    now rewrite term_free11.
-  Qed.
-
-  Lemma term_in_freeset12 : forall (y : atom) (x : atom),
-      AtomSet.In x (freeset (tvar (Fr y))) <-> x = y.
-  Proof.
-    intros. rewrite <- free_iff_freeset.
-    now rewrite term_free12.
-  Qed.
-
-  Lemma term_in_freeset2 : forall (x : atom) (t : term LN) (X : typ),
-      AtomSet.In x (freeset (lam X t)) <-> AtomSet.In x (freeset t).
-  Proof.
-    intros. rewrite <- 2(free_iff_freeset). now rewrite term_free2.
-  Qed.
-
-  Lemma term_in_freeset3 : forall (x : atom) (t1 t2 : term LN),
-      AtomSet.In x (freeset (app t1 t2)) <-> AtomSet.In x (freeset t1) \/ AtomSet.In x (freeset t2).
-  Proof.
-    intros. rewrite <- 3(free_iff_freeset). now rewrite term_free3.
-  Qed.
-
-  Open Scope set_scope.
-
-  Lemma term_freeset11 : forall (b : nat) (x : atom),
-      freeset (tvar (Bd b)) [=] ∅.
-  Proof.
-    intros. fsetdec.
-  Qed.
-
-  Lemma term_freeset12 : forall (y : atom),
-      freeset (tvar (Fr y)) [=] {{ y }}.
-  Proof.
-    intros. cbn. fsetdec.
-  Qed.
-
-  Lemma term_freeset2 : forall (t : term LN) (X : typ),
-      freeset (lam X t) [=] freeset t.
-  Proof.
-    intros. unfold AtomSet.Equal; intro x.
-    rewrite term_in_freeset2. reflexivity.
-  Qed.
-
-  Lemma term_freeset3 : forall (t1 t2 : term LN),
-      freeset (app t1 t2) [=] freeset t1 ∪ freeset t2.
-  Proof.
-    intros. unfold AtomSet.Equal; intro x.
-    rewrite term_in_freeset3. fsetdec.
-  Qed.
-
-End term_free_rewrite.
-
-(** ** Rewriting lemmas for <<foldMapd>> *)
-(******************************************************************************)
-Section term_foldMapd_rewrite.
-
-  Context {A M : Type} (f : nat * A -> M) `{Monoid M}.
-
-  Lemma term_foldMapd1 : forall (a : A),
-      foldMapd f (tvar a) = f (Ƶ, a).
-  Proof.
-    reflexivity.
-  Qed.
-
-  Lemma term_foldMapd2 : forall X (t : term A),
-      foldMapd f (λ X t) = foldMapd (preincr f 1) t.
-  Proof.
-    intros. cbv. change (op unit0 ?f) with (Ƶ ● f).
-    now simpl_monoid.
-  Qed.
-
-  Lemma term_foldMapd3 : forall (t1 t2 : term A),
-      foldMapd f ([t1]@[t2]) = foldMapd f t1 ● foldMapd f t2.
-  Proof.
-    intros. cbv. change (op unit0 ?f) with (Ƶ ● f).
-    now simpl_monoid.
-  Qed.
-
-End term_foldMapd_rewrite.
-
-(** ** Rewriting lemmas for <<∈d>> *)
-(******************************************************************************)
-Section term_ind_rewrite.
-
-  Lemma term_ind1 : forall (l1 l2 : LN) (n : nat),
-      (n, l1) ∈d (tvar l2) <-> n = Ƶ /\ l1 = l2.
-  Proof.
-    introv.
-    rewrite ctx_elements_to_foldMapd.
-    rewrite term_foldMapd1.
-    split.
-    - now inversion 1.
-    - inversion 1. now subst.
-  Qed.
-
-  Lemma term_ind2 : forall (t : term LN) (l : LN) (n : nat) (X : typ),
-      (n, l) ∈d t = (S n, l) ∈d (λ X t).
-  Proof.
-    intros.
-    rewrite ctx_elements_to_foldMapd.
-    rewrite (term_foldMapd2 _).
-    change_left ((evalAt (n, l) ∘ foldMapd (ret (T := subset))) t).
-    rewrite foldMapd_morphism.
-    change_right ((evalAt (S n, l) ∘ foldMapd (ret (T := subset) ⦿ 1)) t).
-    rewrite foldMapd_morphism.
-    fequal.
-    ext [n' l'].
-    cbv.
-    propext.
-    now inversion 1.
-    now inversion 1.
-  Qed.
-
-  Lemma term_ind2' : forall (t : term LN) (l : LN) (n : nat) (X : typ),
-      (n, l) ∈d (λ X t) = ((n - 1, l) ∈d t /\ n <> 0).
-  Proof.
-    intros.
-    rewrite ctx_elements_to_foldMapd.
-    rewrite (term_foldMapd2 _).
-    change_left ((evalAt (n, l) ∘ foldMapd (ret (T := subset) ⦿ 1)) t).
-    rewrite foldMapd_morphism.
-    change_right ((evalAt (n-1, l) ∘ foldMapd (ret (T := subset))) t /\ n <> 0).
-    rewrite foldMapd_morphism.
-    (*
-    assert (evalAt (n, l) ∘ ret ⦿ 1 = (evalAt (n - 1, l) ∘ ret /\ n <> 0)).
-    { unfold evalAt, preincr, incr, ret, Return_subset, compose.
-      unfold_ops @Monoid_op_plus.
-      propext.
-      apply propositional_extensionality.
-      ext [n' l'].
-      propext.
-      - inversion 1. cbn.
-        assert (n <> 0).
-        lia. fequal. lia.
-      - inversion 1. cbn.
-        fequal.
-     *)
-  Admitted.
-
-  Lemma term_ind3 : forall (t1 t2 : term LN) (n : nat) (l : LN),
-      (n, l) ∈d ([t1]@[t2]) <-> (n, l) ∈d t1 \/ (n, l) ∈d t2.
-  Proof.
-    introv.
-    rewrite ctx_elements_to_foldMapd.
-    rewrite (term_foldMapd3 _).
-    reflexivity.
-  Qed.
-
-End term_ind_rewrite.
-
-(** ** Rewriting lemmas for <<subst>> *)
-(******************************************************************************)
-
-(** ** Rewriting lemmas for <<locally_closed>> *)
-(******************************************************************************)
-Theorem term_lc_gap11 : forall (n : nat) (m : nat),
-    locally_closed_gap m (tvar (Bd n)) <-> n < m.
+Theorem dtm4_stlc :
+  forall (G1 G2 : Type -> Type) (H1 : Map G1) (H2 : Mult G1) (H3 : Pure G1) (H4 : Map G2) (H5 : Mult G2) (H6 : Pure G2)
+    (ϕ : forall A : Type, G1 A -> G2 A), ApplicativeMorphism G1 G2 ϕ ->
+                                   forall (A B : Type) (f : nat * A -> G1 (term B)),
+                                     ϕ (term B) ∘ binddt f = binddt (ϕ (term B) ∘ f).
 Proof.
-  intros. unfold locally_closed_gap.
-  split.
-  - intros. specialize (H 0 (Bd n)).
-    rewrite term_ind1 in H. specialize (H (ltac:(intuition))).
-    apply H.
-  - intros. cbn. rewrite term_ind1 in H0. destruct H0; subst.
-    now simpl_monoid.
-Qed.
-
-Theorem term_lc_gap12 : forall (x : atom) (m : nat),
-    locally_closed_gap m (tvar (Fr x)) <-> True.
-Proof.
-  intros. unfold locally_closed, locally_closed_gap.
-  setoid_rewrite term_ind1. intuition.
-  now subst.
-Qed.
-
-Theorem term_lc_gap2 : forall (X : typ) (t : term LN) (m : nat),
-    locally_closed_gap m (lam X t) <-> locally_closed_gap (S m) t.
-Proof.
-  intros. unfold locally_closed, locally_closed_gap.
-  setoid_rewrite term_ind2'. split.
-  - introv premise hypothesis. destruct l; [easy|].
-    cbn. specialize (premise (S w) (Bd n)).
-    cbn in premise.
-    replace (w - 0) with w in premise by lia.
-    assert (H : S w <> 0) by lia.
-    specialize (premise (conj hypothesis H)).
-    unfold_lia.
-  - introv premise [hypothesis neq0].
-    destruct l; [easy|].
-    specialize(premise (w - 1) (Bd n) hypothesis).
-    cbn in *. unfold_lia.
-Qed.
-
-Theorem term_lc_gap3 : forall (t1 t2 : term LN) (m : nat),
-    locally_closed_gap m ([t1]@[t2]) <-> locally_closed_gap m t1 /\ locally_closed_gap m t2.
-Proof.
-  intros. unfold locally_closed, locally_closed_gap.
-  setoid_rewrite term_ind3. intuition.
-Qed.
-
-Theorem term_lc11 : forall (n : nat),
-    locally_closed (tvar (Bd n)) <-> False.
-Proof.
-  intros. unfold locally_closed. now (rewrite term_lc_gap11).
-Qed.
-
-Theorem term_lc12 : forall (x : atom),
-    locally_closed (tvar (Fr x)) <-> True.
-Proof.
-  intros. unfold locally_closed. now (rewrite term_lc_gap12).
-Qed.
-
-Theorem term_lc2 : forall (X : typ) (t : term LN),
-    locally_closed (lam X t) <-> locally_closed_gap 1 t.
-Proof.
-  intros. unfold locally_closed. now (rewrite term_lc_gap2).
-Qed.
-
-Theorem term_lc3 : forall (t1 t2 : term LN),
-    locally_closed ([t1]@[t2]) <-> locally_closed t1 /\ locally_closed t2.
-Proof.
-  intros. unfold locally_closed.
-  now setoid_rewrite term_lc_gap3.
-Qed.
+  intros. ext t.
+  inversion H.
+  generalize dependent f.
+  unfold compose at 1.
+  induction t; intro f. (* .unfold *)
+  - reflexivity.
+  - cbn.
+    repeat rewrite ap_morphism_1.
+    rewrite appmor_pure.
+    rewrite IHt.
+    admit.
+  - cbn.
+    repeat rewrite ap_morphism_1.
+    rewrite appmor_pure.
+    rewrite IHt1.
+    rewrite IHt2.
+    reflexivity.
+Abort.
